try to extract mpfr

code/experimental/mpfr/include/MPFR_Lib_Clz.c
@@ -1,0 +1,6 @@
+#include "MPFR_Lib_Clz.h"
+
+uint32_t MPFR_Lib_Clz_count_leading_zeros (uint64_t a) {
+  return __builtin_clz(a);
+}
+
