code/experimental/mpfr/include/MPFR_Lib_Clz.h
@@ -1,0 +1,4 @@
+#include "inttypes.h"
+
+uint32_t MPFR_Lib_Clz_count_leading_zeros (uint64_t a);
+
