code/experimental/mpfr/MPFR.Add1sp1.Lemma.fst
@@ -9,9 +9,9 @@ open FStar.UInt64
 open FStar.Int.Cast
 open FStar.Mul
 open MPFR.Lib
-open MPFR.Lib.Spec
-open MPFR.Add1.Spec
-open MPFR.Round.Spec
+open MPFR.Spec.Lib
+open MPFR.Spec.Add1
+open MPFR.Spec.Round
 open MPFR.Dyadic
 open MPFR.Maths
 
@@ -71,7 +71,6 @@ val mpfr_add1sp1_gt_branch12_a0_bx_lemma:
     v a0 = r.limb / pow2 (r.len - 64) /\ I64.v bx = r.exp))
 
 let mpfr_add1sp1_gt_branch12_a0_bx_lemma h a b c sh d mask =
-    admit();
     let r = add1sp_exact (as_reg_fp_ h b) (as_reg_fp_ h c) in
     let bx = b.mpfr_exp in
     let b0 = Seq.index (as_seq h b.mpfr_d) 0 in
@@ -117,7 +116,6 @@ val mpfr_add1sp1_gt_branch12_value_lemma:
     let bx = b.mpfr_exp in
     let b0 = Seq.index (as_seq h bp) 0 in
     let c0 = Seq.index (as_seq h cp) 0 in
-    admit();
     let a0 = b0 +%^ (c0 >>^ (int64_to_uint32 d)) in
     let a0, bx = if a0 <^ b0 then mpfr_LIMB_HIGHBIT |^ (a0 >>^ 1ul), I64.(bx +^ 1L) else a0, bx in
     let a0 = a0 &^ (lognot mask) in
@@ -132,7 +130,6 @@ let mpfr_add1sp1_gt_branch12_value_lemma h a b c sh d mask =
     let bx = b.mpfr_exp in
     let b0 = Seq.index (as_seq h bp) 0 in
     let c0 = Seq.index (as_seq h cp) 0 in
-    admit();
     let a0 = b0 +%^ (c0 >>^ (int64_to_uint32 d)) in
     let t0 = v b0 + v c0 / pow2 (I64.v d) in
     let a0, bx = if a0 <^ b0 then mpfr_LIMB_HIGHBIT |^ (a0 >>^ 1ul), I64.(bx +^ 1L) else a0, bx in
@@ -498,12 +495,10 @@ val mpfr_add1sp1_eq_value_lemma:
     let bx = I64.(b.mpfr_exp +^ 1L) in
     let rb = a0 &^ (mpfr_LIMB_ONE <<^ (int64_to_uint32 I64.(sh -^ 1L))) in
     let a0 = a0 ^^ rb in
-    admit();
     v a0 * pow2 (r.len - 64) = r.limb /\ I64.v bx = r.exp /\
     v a0 >= pow2 63 /\ v a0 % pow2 (64 - p) = 0))
-
+    
 let mpfr_add1sp1_eq_value_lemma h a b c sh =
-    admit();
     let p = I64.v a.mpfr_prec in
     let r = add1sp_exact (as_reg_fp_ h b) (as_reg_fp_ h c) in
     let bp = b.mpfr_d in
@@ -731,6 +726,8 @@ val mpfr_ternary_cond_lemma: a:normal_fp{mpfr_EXP_COND a.exp} ->
                t = mpfr_add1sp1_ternary_spec high rb sb rnd_mode))
     (ensures  (mpfr_ternary_cond t a r))
 
+#set-options "--z3rlimit 4000" 
+
 let mpfr_ternary_cond_lemma a p high rb sb rnd_mode t r =
     if ((high_mant a p).len>=high.len) then begin
        lemma_pow2_sub high.limb (high_mant a p).limb (high_mant a p).len high.len
@@ -751,8 +748,10 @@ let mpfr_ternary_cond_lemma a p high rb sb rnd_mode t r =
         mpfr_truncate_ternary_cond_lemma a p high rb sb rnd_mode t r
     else begin
         rb_sb_lemma a p;
-        mpfr_add_one_ulp_ternary_cond_lemma a p high rnd_mode t r;admit() (*How is this non-obvious ?*)
+        mpfr_add_one_ulp_ternary_cond_lemma a p high rnd_mode t r
     end
+
+#set-options "--z3rlimit 100"
 
 val mpfr_add1sp1_round_post_cond_lemma: a:normal_fp{mpfr_EXP_COND a.exp} ->
     p:pos{mpfr_PREC_COND p} ->
