code/experimental/mpfr/MPFR.fst
@@ -2,4 +2,4 @@ module MPFR
 
 let mpfr_add1sp1 = MPFR.Add1sp1.mpfr_add1sp1 
 let mpfr_mul_1 = MPFR.Mul_1.mpfr_mul_1
-//let mpfr_sub1sp1 = MPFR.Sub1sp1.mpfr_sub1sp1
+let mpfr_sub1sp1 = MPFR.Sub1sp1.mpfr_sub1sp1
