code/experimental/mpfr/MPFR.Lib.Clz.fsti
@@ -1,0 +1,27 @@
+module MPFR.Lib.Clz
+
+open FStar.Mul
+open FStar.UInt64
+open FStar.UInt
+
+open MPFR.Dyadic
+open MPFR.Spec.Lib
+open MPFR.Spec.Sub1
+open MPFR.Spec.Round
+open MPFR.Maths
+
+open MPFR.Lib
+open MPFR.Exceptions
+
+open MPFR.Exceptions.Lemma
+open MPFR.Sub1sp1.Lemma
+open MPFR.Add1sp1
+open MPFR.Add1sp1.Lemma
+
+
+module U32 = FStar.UInt32
+
+
+inline_for_extraction
+val count_leading_zeros:
+  a:u64{not (a=^0uL)} -> Tot (cnt:u32{U32.v cnt<32 /\ v (a<<^cnt)>=pow2 63 /\ v a*pow2 (U32.v cnt)<pow2 64 /\ U32.v cnt=64-(nbits (v a))})
