code/experimental/mpfr/MPFR.Sub1sp1.Lemma.fst
@@ -1,0 +1,494 @@
+module MPFR.Sub1sp1.Lemma
+
+open FStar.HyperStack.All
+open FStar.HyperStack
+open FStar.HyperStack.ST
+open FStar.Buffer
+open FStar.UInt64
+open FStar.UInt
+open FStar.Int.Cast
+open FStar.Mul
+open MPFR.Dyadic
+open MPFR.Spec.Lib
+open MPFR.Spec.Sub1
+open MPFR.Spec.Round
+open MPFR.Maths
+
+open MPFR.Lib
+open MPFR.Exceptions
+
+open MPFR.Exceptions.Lemma
+open MPFR.Add1sp1
+open MPFR.Add1sp1.Lemma
+
+module ST = FStar.HyperStack.ST
+module I32 = FStar.Int32
+module I64 = FStar.Int64
+module U32 = FStar.UInt32
+
+#set-options "--z3refresh --z3rlimit 100 --max_fuel 1 --initial_fuel 0 --max_ifuel 1 --initial_ifuel 0"
+
+private type mpfr_tmp_exp_t = x:mpfr_exp_t{I64.((*x >=^ mpfr_EMIN /\*) x <=^ mpfr_EMAX +^ 1L)}
+
+let mpfr_sub1sp1_pre_cond h (a:mpfr_ptr) b c (p:mpfr_prec_t): GTot Type0=
+        (* Memory safety *)
+        mpfr_live h a /\ mpfr_live h b /\ mpfr_live h c /\
+        mpfr_disjoint_or_equal h a b /\ mpfr_disjoint_or_equal h a c /\
+        mpfr_disjoint_or_equal h b c /\
+        length (as_struct h a).mpfr_d = 1 /\
+        length (as_struct h b).mpfr_d = 1 /\ length (as_struct h c).mpfr_d = 1 /\
+        (* Functional correctness *)
+        I64.v p > 0 /\ I64.v p < 64 /\ p = (as_struct h a).mpfr_prec /\
+        p = (as_struct h b).mpfr_prec /\ p = (as_struct h c).mpfr_prec /\
+        mpfr_valid_cond h a /\ mpfr_reg_cond h b /\ mpfr_reg_cond h c
+
+let mpfr_sub1sp1_pre_cond_2 h (a:mpfr_ptr) b c bx cx ap bp cp p sh: GTot Type0=
+ (as_struct h b).mpfr_exp=bx /\
+ (as_struct h c).mpfr_exp=cx /\ 
+ (as_struct h a).mpfr_d==ap /\
+ (as_struct h b).mpfr_d==bp /\
+ (as_struct h c).mpfr_d==cp /\
+ live h ap /\ live h bp /\ live h cp /\
+ I64.v sh = I64.v gmp_NUMB_BITS - I64.v p
+
+val lemma_shift_left_mod_pow2: a:t -> s:U32.t -> k:nat -> Lemma
+  (requires ((v a)%(pow2 k)=0)/\U32.v s<64 /\ k<64)//could be proven without the k<64 condition
+  (ensures ((v (a<<^s))%(pow2 k)=0))
+  
+let lemma_shift_left_mod_pow2 a s k=
+   shift_left_value_lemma (v a) U32.(v s);//a<<^s=(a*2^s)%(2^64)
+   lemma_pow2_mod_mod (v a*pow2 U32.(v s)) 64 k;//a<<^s%(2^k)=a*(2^s)%(2^k)
+   lemma_mul_mod_zero (v a) (pow2 U32.(v s)) (pow2 k)
+
+val mpfr_sub1sp1_eq_rb_sb_lemma:
+    b:mpfr_reg_fp -> c:mpfr_reg_fp -> p:pos -> Lemma
+    (requires (
+    b.prec=p /\ c.prec=p /\
+    b.exp=c.exp /\
+    b.limb<>c.limb
+    ))
+    (ensures (let r = sub1sp_exact b c in rb_def r p=false /\ sb_def r p=false))
+    
+let mpfr_sub1sp1_eq_rb_sb_lemma b c p=
+    let r=sub1sp_exact b c in
+    let b,c=if gt (eval_abs c) (eval_abs b) then c,b else b,c in
+    assert(pow2 (b.exp-c.exp)=1);
+    lemma_mod_distr_sub_zero (b.limb * pow2 (b.exp - c.exp)) c.limb (pow2 (c.len-c.prec));
+    lemma_pow2_gt_rev (sub1sp_gt_len b c) (c.len-c.prec);
+    assert(b.limb>=r.limb \/ c.limb>=r.limb);
+    assert(pow2 b.len>=r.limb);
+    assert(pow2 b.len>pow2 (r.len-1));
+    lemma_pow2_gt_rev b.len (r.len-1);
+    assert(r.limb%pow2 (b.len-b.prec)=0);
+    if(p<r.prec) then (rb_value_lemma r p;
+      lemma_pow2_mod_mod_zero r.limb (b.len-b.prec) (r.len-p-1);
+      lemma_pow2_mod_mod_zero r.limb (b.len-b.prec) (r.len-p))
+
+val lemma_fp_eq_cross:
+    a:valid_fp -> b:valid_fp ->Lemma
+    (requires (eval_abs a =. eval_abs b /\ a.exp=b.exp))
+    (ensures (a.limb*pow2 b.len=b.limb*pow2 a.len)) 
+
+let lemma_fp_eq_cross a b=
+    let da,db=eval a,eval b in
+    let elb=min da.exponent db.exponent in
+    assert(a.limb*pow2(a.exp-a.len-elb)=b.limb*pow2(b.exp-b.len-elb));
+    assert(a.limb*pow2(a.exp-a.len-elb)*pow2 a.len=b.limb*pow2 a.len*pow2(b.exp-b.len-elb));
+    lemma_pow2_mul (a.exp-a.len-elb) a.len;
+    assert(a.limb*pow2(a.exp-elb)=b.limb*pow2 a.len*pow2(b.exp-b.len-elb));
+    assert(a.limb*pow2 b.len*pow2(a.exp-elb)=b.limb*pow2 a.len*pow2(b.exp-b.len-elb)*pow2 b.len);
+    lemma_paren_mul_right (b.limb*pow2 a.len) (pow2 (b.exp-b.len-elb)) (pow2 b.len);
+    lemma_pow2_mul (b.exp-b.len-elb) b.len;
+    assert(a.limb*pow2 b.len*pow2(a.exp-elb)=(b.limb*pow2 a.len)*pow2(b.exp-elb));
+    lemma_mul_simp (a.limb*pow2 b.len) (b.limb*pow2 a.len) (pow2 (a.exp-elb))
+
+val mpfr_sub1sp1_eq_value_lemma:
+    a:normal_fp -> b:mpfr_reg_fp -> c:mpfr_reg_fp -> cnt:nat -> p:pos -> Lemma
+    (requires (
+    b.prec=p /\ c.prec=p /\ p<64 /\
+    b.exp=c.exp /\
+    b.limb<>c.limb /\
+    (let b,c=if gt (eval_abs c) (eval_abs b) then c,b else b,c in
+    cnt=64-(nbits (b.limb-c.limb)) /\
+    a.limb=(b.limb-c.limb)*pow2 cnt /\
+    a.exp=b.exp-cnt /\
+    a.len=64
+    ) ))
+    (ensures (let r = sub1sp_exact b c in  a.limb * pow2 (high_mant r p).len = (high_mant r p).limb * (pow2 64) /\ a.exp = (high_mant r p).exp))
+
+let mpfr_sub1sp1_eq_value_lemma a b c cnt p=
+    let r=sub1sp_exact b c in
+    let b,c=if gt (eval_abs c) (eval_abs b) then c,b else b,c in
+    let k=high_mant r p in
+    assert(a.exp=k.exp);
+    assert(eval_abs a=.eval_abs r);
+    if p<=r.prec then begin 
+      assert(r.len<b.len);
+      lemma_pow2_lt (r.len-p) (b.len-p);
+      assert(b.limb%pow2(b.len-p)=0);
+      assert(c.limb%pow2(b.len-p)=0);
+      lemma_mod_distr_sub_zero b.limb c.limb (pow2 (b.len-p));
+      assert(r.limb%pow2(b.len-p)=0);
+      lemma_pow2_mod_mod_zero r.limb (b.len-p) (r.len-p);
+      assert(r.limb%pow2(r.len-p)=0);
+      lemma_div_mul r.limb (pow2 (r.len-p));
+      assert(r.limb=k.limb)
+    end;
+    assert(eval_abs r=.eval_abs k);
+    lemma_fp_eq_cross a k
+
+val lemma_gt_exp_sub1sp:  b:mpfr_reg_fp -> c:mpfr_reg_fp -> Lemma
+ (requires (b.exp>c.exp))
+ (ensures (gt (eval_abs b) (eval_abs c)))
+
+let lemma_gt_exp_sub1sp b c=
+    let eb,ec=(eval_abs b),(eval_abs c) in
+    let elb=min eb.exponent ec.exponent in
+    assert(b.limb>=pow2 (b.len-1));
+    assert(b.limb*(pow2 (b.exp-b.len-elb))>=pow2 (b.len-1)*(pow2 (b.exp-b.len-elb)));
+    lemma_pow2_mul (b.len-1) (b.exp-b.len-elb);
+    assert(b.limb*(pow2 (b.exp-b.len-elb))>=pow2 (b.exp-1-elb));
+    assert(pow2 c.len>c.limb);
+    lemma_pow2_le (c.exp-elb) (b.exp-1-elb);
+    assert(pow2 (b.exp-1-elb)>=pow2 (c.exp-elb));
+    lemma_pow2_mul c.len (c.exp-c.len-elb);
+    assert(b.limb*(pow2 (b.exp-b.len-elb))>c.limb*pow2 (c.exp-c.len-elb))
+
+val lemma_sub1sp1_gt_exp_2_limb1: b:mpfr_reg_fp -> c:mpfr_reg_fp -> p:pos{b.prec=p /\ c.prec=p /\ p<64} -> Lemma
+    (requires (b.exp>c.exp /\ b.exp-c.exp>=64 /\ b.limb<>v mpfr_LIMB_HIGHBIT))
+    (ensures (let r=sub1sp_exact b c in
+        let d=b.exp-c.exp in
+        r.limb>=pow2 (63+d)
+    ))
+
+let lemma_sub1sp1_gt_exp_2_limb1 b c p=
+    lemma_gt_exp_sub1sp b c;
+    let d=b.exp-c.exp in
+    let r=sub1sp_exact b c in
+    assert(r.limb=b.limb*pow2 d-c.limb);
+    assert(c.limb<pow2 c.len);
+    assert(c.len<=d);
+    lemma_pow2_le c.len d;
+    assert(r.limb>=(b.limb-1)*pow2 d);
+    assert(b.limb-1>=pow2 63);
+    lemma_pow2_mul 63 d;
+    lemma_mul_le_left (pow2 d) (pow2 63) (b.limb-1);
+    assert(r.limb>=pow2 (63+d))
+
+val lemma_sub1sp1_gt_exp_2_limb2: b:mpfr_reg_fp -> c:mpfr_reg_fp -> p:pos{b.prec=p /\ c.prec=p /\ p<64} -> Lemma
+    (requires (b.exp>c.exp /\ b.exp-c.exp>=64 /\ b.limb<>v mpfr_LIMB_HIGHBIT))
+    (ensures (let r=sub1sp_exact b c in
+        let d=b.exp-c.exp in
+        r.limb<pow2 (64+d)
+    ))
+
+let lemma_sub1sp1_gt_exp_2_limb2 b c p=
+    lemma_gt_exp_sub1sp b c;
+    let d=b.exp-c.exp in
+    let r=sub1sp_exact b c in
+    assert(r.limb=b.limb*pow2 d-c.limb);
+    assert(r.limb<=b.limb*pow2 d);
+    assert(b.limb<pow2 b.len);
+    assert(b.len=64);
+    lemma_pow2_mul 64 d;
+    assert(r.limb<pow2 (64+d))
+
+val lemma_sub1sp1_gt_rb_sb_exp_2:  b:mpfr_reg_fp -> c:mpfr_reg_fp -> p:pos{b.prec=p /\ c.prec=p /\ p<64} -> Lemma
+    (requires (b.exp>c.exp /\ b.exp-c.exp>=64 /\ b.limb<>v mpfr_LIMB_HIGHBIT))
+    (ensures (let r=sub1sp_exact b c in
+        r.exp=b.exp /\ rb_def r p /\ sb_def r p
+    ))
+
+let lemma_sub1sp1_gt_rb_sb_exp_2 b c p=
+    lemma_gt_exp_sub1sp b c;
+    let d=b.exp-c.exp in
+    let r=sub1sp_exact b c in
+    lemma_sub1sp1_gt_exp_2_limb1 b c p;
+    lemma_sub1sp1_gt_exp_2_limb2 b c p;
+    lemma_pow2_nbits_rev r.limb (64+d);
+    (*sb*)
+    lemma_pow2_le 64 (r.len-p-1);
+    lemma_small_mod c.limb (pow2 (r.len - p - 1));
+    let cm=c.limb % pow2 (r.len - p - 1) in
+    lemma_pow2_mod_mod_zero b.limb (64-p) (r.len-p-d);
+    lemma_mod_mul b.limb (pow2 (r.len-p-d)) (pow2 d);
+    lemma_pow2_mul (r.len-p-d) d;
+    lemma_pow2_mod_mod_zero (b.limb*pow2 d) (r.len-p) (r.len-p-1);
+    lemma_mod_distr_sub (b.limb * pow2 d) c.limb (pow2 (r.len - p - 1));
+    (*rb*)
+    lemma_pow2_le 64 (r.len-p);
+    lemma_small_mod c.limb (pow2 (r.len - p));
+    lemma_mod_distr_sub (b.limb * pow2 d) c.limb (pow2 (r.len - p));
+    lemma_small_mod_neg cm (pow2 (r.len - p));
+    lemma_small_mod_neg cm (pow2 (r.len - p-1));
+    rb_value_lemma r p
+
+val lemma_sub1sp1_gt_value_2:  b:mpfr_reg_fp -> c:mpfr_reg_fp -> p:pos{b.prec=p /\ c.prec=p /\ p<64} -> Lemma
+    (requires (b.exp>c.exp /\ b.exp-c.exp>=64 /\ b.limb<>v mpfr_LIMB_HIGHBIT))
+    (ensures (let r=sub1sp_exact b c in
+       (b.limb-(pow2 (64-p))) * pow2 (high_mant r p).len = (high_mant r p).limb * (pow2 64)
+    ))
+
+let lemma_sub1sp1_gt_value_2 b c p=
+    lemma_gt_exp_sub1sp b c;
+    let d=b.exp-c.exp in
+    let r=sub1sp_exact b c in
+    lemma_sub1sp1_gt_exp_2_limb1 b c p;
+    lemma_sub1sp1_gt_exp_2_limb2 b c p;
+    lemma_pow2_nbits_rev r.limb (64+d);
+    lemma_pow2_mod_mod_zero b.limb (64-p) (r.len-p-d);
+    lemma_mod_mul b.limb (pow2 (r.len-p-d)) (pow2 d);
+    lemma_pow2_mul (r.len-p-d) d;
+    lemma_pow2_le 64 (r.len-p);
+
+    lemma_pow2_mul (r.len-64) (64-p);
+    lemma_div_div (b.limb*pow2 d) (pow2 d) (pow2 (64-p));
+    lemma_multiple_div b.limb (pow2 d);
+    //!  assert((b.limb*pow2 d)/(pow2 (r.len-p))=b.limb/(pow2 (64-p)));
+    lemma_small_div_neg c.limb (pow2 (r.len - p));
+    lemma_div_distr (b.limb*pow2 d) (0-c.limb) (pow2 (r.len-p));
+    //! assert((high_mant r p).limb*(pow2 64)=(b.limb / pow2 (64 - p) - 1)*(pow2 (r.len-p))*(pow2 64));
+    lemma_paren_mul_right (b.limb / pow2 (64 - p) - 1) (pow2 (r.len-p)) (pow2 64);
+    lemma_pow2_mul (r.len-p) 64;
+    lemma_paren_mul_right (b.limb / pow2 (64 - p) - 1) (pow2 (64-p)) (pow2 r.len);
+    lemma_pow2_mul r.len (64-p);
+    //! assert((high_mant r p).limb*(pow2 64)=((b.limb / pow2 (64 - p) - 1)*(pow2 (64-p)))*pow2 r.len);
+    lemma_distr_sub_left (b.limb/pow2 (64-p)) 1 (pow2 (64-p));
+    lemma_div_mul b.limb (pow2 (64-p))
+  
+
+val lemma_sub1sp1_gt_rb_sb_exp_3:  b:mpfr_reg_fp -> c:mpfr_reg_fp -> p:pos{b.prec=p /\ c.prec=p /\ p<64} -> Lemma
+    (requires (b.exp>c.exp /\ b.exp-c.exp>=64 /\ b.limb=v mpfr_LIMB_HIGHBIT))
+    (ensures (let r=sub1sp_exact b c in
+        r.exp=b.exp-1 /\ 
+        rb_def r p=(p<63||b.exp-c.exp>64||c.limb=v mpfr_LIMB_HIGHBIT) /\
+        sb_def r p=(p<63||b.exp-c.exp>64||c.limb<>v mpfr_LIMB_HIGHBIT)
+    ))
+
+let lemma_sub1sp1_gt_rb_sb_exp_3 b c p=
+    lemma_gt_exp_sub1sp b c;
+    let d=b.exp-c.exp in
+    let r=sub1sp_exact b c in
+    lemma_pow2_mul 63 d;
+    lemma_pow2_le 64 (62+d);
+    lemma_pow2_nbits_rev r.limb (63+d);
+    
+    lemma_mod_product_zero b.limb (pow2 d) (pow2 (64-p)) (pow2 d);
+    lemma_pow2_mul (64-p) d;
+    
+    lemma_pow2_mod_mod_zero (b.limb*pow2 d) (64-p+d) (62+d-p);
+    lemma_small_mod 0 (pow2 (62+d-p));
+    lemma_mod_distr_sub (b.limb*pow2 d) c.limb (pow2 (62+d-p));
+    lemma_mod_distr_sub 0 c.limb (pow2 (62+d-p));
+
+    lemma_pow2_mod_mod_zero (b.limb*pow2 d) (64-p+d) (63+d-p);
+    lemma_small_mod 0 (pow2 (63+d-p));
+    lemma_mod_distr_sub (b.limb*pow2 d) c.limb (pow2 (63+d-p));
+    lemma_mod_distr_sub 0 c.limb (pow2 (63+d-p));
+
+    rb_value_lemma r p;
+    if p<63||d>64 then begin
+      lemma_pow2_le 64 (62+d-p);
+      lemma_small_mod_neg c.limb (pow2 (62+d-p));
+      lemma_pow2_le 64 (63+d-p);
+      lemma_small_mod_neg c.limb (pow2 (63+d-p))
+    end
+
+val lemma_sub1sp1_gt_value_3:  b:mpfr_reg_fp -> c:mpfr_reg_fp -> p:pos{b.prec=p /\ c.prec=p /\ p<64} -> Lemma
+    (requires (b.exp>c.exp /\ b.exp-c.exp>=64 /\ b.limb=v mpfr_LIMB_HIGHBIT))
+    (ensures (let r=sub1sp_exact b c in
+       (pow2 64-pow2 (64-p)) * pow2 (high_mant r p).len = (high_mant r p).limb * (pow2 64)
+    ))
+
+let lemma_sub1sp1_gt_value_3 b c p=
+    lemma_gt_exp_sub1sp b c;
+    let d=b.exp-c.exp in
+    let r=sub1sp_exact b c in
+    lemma_pow2_mul 63 d;
+    lemma_pow2_le 64 (62+d);
+    lemma_pow2_nbits_rev r.limb (63+d);
+    
+    lemma_mod_product_zero b.limb (pow2 d) (pow2 (64-p)) (pow2 d);
+    lemma_pow2_mul (64-p) d;
+
+    lemma_pow2_mod_mod_zero (b.limb*pow2 d) (64-p+d) (63+d-p);
+    lemma_small_mod 0 (pow2 (63+d-p));
+    
+    lemma_div_distr (b.limb*pow2 d) (0-c.limb) (pow2 (63+d-p));
+    lemma_pow2_mul (63+d-p) p;
+    lemma_multiple_div (pow2 p) (pow2 (63+d-p));
+    lemma_pow2_le 64 (63+d-p);
+    lemma_small_div_neg c.limb (pow2 (63+d-p));
+    lemma_distr_sub_left (pow2 p) 1 (pow2 (63+d-p));
+    lemma_distr_sub_left (pow2 (63+d)) (pow2 (63+d-p)) (pow2 64);
+    lemma_distr_sub_left (pow2 (64)) (pow2 (64-p)) (pow2 (63+d));
+    lemma_pow2_mul (63+d-p) 64;
+    lemma_pow2_mul (64-p) (63+d)
+    
+val lemma_sub1sp1_gt_1_valid: bp:mp_limb_t -> cp:mp_limb_t -> d:I64.t{I64.(0L<^d /\ d<^64L)} -> Lemma
+    (requires (v bp>=pow2 63 /\ (v cp)%2=0))
+    (ensures (let sb=UInt64.minus (cp<<^(int64_to_uint32 I64.(gmp_NUMB_BITS -^ d))) in
+    bp -^ (if sb=^0uL then 0uL else 1uL)>^(cp >>^ (int64_to_uint32 d)) ))
+
+let lemma_sub1sp1_gt_1_valid bp cp d=
+    let sb=UInt64.minus (cp<<^(int64_to_uint32 I64.(gmp_NUMB_BITS -^ d))) in
+    if (I64.v d)=1 then begin
+      shift_left_value_lemma (v cp) 63;
+      lemma_minus_eq_zero_sub (v (cp<<^(int64_to_uint32 I64.(gmp_NUMB_BITS -^ d))))
+    end else begin
+      shift_right_value_lemma (v cp) (I64.v d);
+      lemma_div_le (v cp) (pow2 64) (pow2 (I64.v d));
+      lemma_pow2_div 64 (I64.v d);
+      lemma_pow2_le (64-(I64.v d)) 62;
+      assert(v (cp >>^ (int64_to_uint32 d)) <= pow2 62);
+      assert_norm(pow2 62 < pow2 63-1)
+    end
+
+val lemma_sub1sp1_gt_branch_1_high_prec: r:normal_fp -> a0:uint_t 64 -> sb_2:uint_t 64 -> mask:uint_t 64 -> p:pos -> Lemma
+    (requires (0<p /\ p<64 /\ p<r.prec /\ mask=pow2 (64-p)-1 /\ r.len<128 /\ a0*pow2 64+sb_2=r.limb*pow2 (128-r.len)))
+    (ensures (
+    let rb=logand a0 (shift_left #64 1 (64-p-1)) in
+    let sb=logor sb_2  (logxor (logand a0 mask) rb) in
+    let ad=logand a0 (lognot mask) in
+    rb_def r p=(rb<>0) /\
+    sb_def r p=(sb<>0) /\
+    ad*pow2 (high_mant r p).len=(high_mant r p).limb*pow2 64
+    ))
+
+let lemma_sub1sp1_gt_branch_1_high_prec r a0 sb_2 mask p=
+    let rb=logand a0 (shift_left #64 1 (64-p-1)) in
+    let sb=logor sb_2  (logxor (logand a0 mask) rb) in
+    let ad=logand a0 (lognot mask) in
+    lemma_pow2_lt (64-p-1) 64;
+    lemma_nth_logand #64 a0 p;
+    lemma_nth_pow2 #64 64 a0 sb_2 p;
+    lemma_nth_pow2 #r.len (128-r.len) r.limb 0 p;
+    assert(rb_def r p=(rb<>0));
+    lemma_mod_mul r.limb (pow2 (r.len-p-1)) (pow2 (128-r.len));
+    lemma_pow2_mul (r.len-p-1) (128-r.len);
+    assert((r.limb%pow2 (r.len-p-1))*pow2 (128-r.len) =(a0*pow2 64+sb_2)%pow2 (128-p-1));
+    assert(sb_def r p=(((a0*pow2 64+sb_2)%pow2 (128-p-1))<>0));
+    assert(128-p-1>=64);
+
+    (if sb=0 then begin
+       logor_ge sb_2  (logxor (logand a0 mask) rb);
+       if((logand a0 mask)<>rb) then logxor_neq_nonzero (logand a0 mask) rb;
+
+       lemma_tl_zero_imp_mod_pow2 rb (64-p-1);
+       logand_mask a0 (64-p);
+
+       lemma_pow2_mul_mod r.limb (128-r.len) (128-p-1);
+       lemma_pow2_mul_mod a0 64 (128-p-1);
+       lemma_pow2_mod_mod a0 (64-p) (64-p-1)
+    end else begin
+      if sb_2<>0 then begin
+         assert(sb_2%pow2 64<>0);
+         assert(((a0*pow2 64+sb_2)%pow2 64)<>0);
+         lemma_pow2_mod_mod (a0*pow2 64+sb_2) (128-p-1) 64
+      end else begin
+        logor_lemma_1 (logxor (logand a0 mask) rb);
+        logor_commutative (logxor (logand a0 mask) rb) sb_2;
+        lemma_pow2_mul_mod a0 64 (128-p-1);
+        nth_lemma (logxor (logand a0 mask) rb) (logand a0 (logxor mask (shift_left #64 1 (64-p-1))));
+        logxor_disjoint_zero #64 (pow2 (64-p-1)) (pow2 (64-p-1)-1) (64-p-1);
+        lemma_pow2_double (64-p-1);
+        logxor_inv #64 (pow2 (64-p-1)-1) (pow2 (64-p-1));
+        logxor_commutative #64 (pow2 (64-p-1)-1) (pow2 (64-p-1));
+        if p=63 then logand_lemma_1 a0
+        else logand_mask a0 (64-p-1)
+      end
+    end);
+    nth_lemma (shift_left (shift_right a0 (64-p)) (64-p)) ad;
+    shift_right_value_lemma a0 (64-p);
+    lemma_euclidean a0 (pow2 (64-p));
+    lemma_multiple_div r.limb (pow2 (128-r.len));
+    lemma_pow2_div_div (a0*pow2 64+sb_2) (128-r.len) (r.len-p);
+    assert(r.limb=(a0*pow2 64+sb_2)/pow2 (128-r.len));
+    lemma_div_distr (a0*pow2 64) sb_2 (pow2 64);
+    assert(a0=(a0*pow2 64+sb_2)/pow2 64);
+    lemma_pow2_div_div (a0*pow2 64+sb_2) 64 (64-p);
+    assert(a0/pow2 (64-p)=(a0*pow2 64+sb_2)/pow2 (128-p));
+    assert(ad=(r.limb/pow2 (r.len-p))*pow2 (64-p));
+    lemma_pow2_mul (64-p) r.len;
+    lemma_pow2_mul (r.len-p) 64;
+    lemma_paren_mul_right (r.limb/pow2 (r.len-p)) (pow2 (64-p)) (pow2 r.len);
+    lemma_paren_mul_right (r.limb/pow2 (r.len-p)) (pow2 (r.len-p)) (pow2 64)
+
+val lemma_sub1sp1_gt_branch_1_rb_sb_value: r:normal_fp -> a0:uint_t 64 -> sb_2:uint_t 64 -> mask:uint_t 64 -> p:pos -> Lemma
+    (requires (0<p /\ p<64 /\ mask=pow2 (64-p)-1 /\ r.len<128 /\ a0*pow2 64+sb_2=r.limb*pow2 (128-r.len)))
+    (ensures (
+    let rb=logand a0 (shift_left #64 1 (64-p-1)) in
+    let sb=logor sb_2  (logxor (logand a0 mask) rb) in
+    let ad=logand a0 (lognot mask) in
+    rb_def r p=(rb<>0) /\
+    sb_def r p=(sb<>0) /\
+    ad*pow2 (high_mant r p).len=(high_mant r p).limb*pow2 64
+    ))
+
+let lemma_sub1sp1_gt_branch_1_rb_sb_value r a0 sb_2 mask p=
+    let rb=logand a0 (shift_left #64 1 (64-p-1)) in
+    let sb=logor sb_2  (logxor (logand a0 mask) rb) in
+    let ad=logand a0 (lognot mask) in
+    if p<r.prec then lemma_sub1sp1_gt_branch_1_high_prec r a0 sb_2 mask p
+    else begin
+      lemma_pow2_mod_product_zero r.limb (pow2 (128-r.len)) (r.len-r.prec) (128-r.len);
+      lemma_pow2_mod_mod_zero (a0*pow2 64+sb_2) (128-r.prec) 64;
+      lemma_add_mod sb_2 a0 (pow2 64);
+      assert(sb_2=0);
+      lemma_pow2_mul (64-r.prec) 64;
+      lemma_mod_mul a0 (pow2 (64-r.prec)) (pow2 64);
+      lemma_pow2_mod_mod_zero a0 (64-r.prec) (64-p);
+
+      lemma_pow2_lt (64-p-1) 64;
+      lemma_nth_logand #64 a0 p;
+      lemma_mod_pow2_imp_tl_zero #64 a0 (64-p);
+      logand_mask a0 (64-p);
+      logxor_self #64 0;
+      logor_self #64 0;
+
+      nth_lemma a0 ad;
+      if p>r.len then begin
+        lemma_pow2_shift a0 r.limb 64 (128-r.len) (p-64);
+        lemma_pow2_mul (p-r.len) 64
+      end else begin
+        lemma_pow2_shift a0 r.limb 64 (128-r.len) (r.len-64)
+      end
+    end
+
+val lemma_sub1sp1_gt_branch_1_a0_bx: b:mpfr_reg_fp -> c:mpfr_reg_fp -> p:pos{b.prec=p /\ c.prec=p /\ p<64} -> sb_1:uint_t 64 -> a0_base:uint_t 64 -> Lemma
+    (requires (b.exp>c.exp /\ b.exp-c.exp<64 /\ sb_1=add_mod #64 (pow2 64-1-(shift_left #64 c.limb (64-(b.exp-c.exp)))) 1 /\ a0_base=(b.limb-(if sb_1=0 then 0 else 1))-(shift_right #64 c.limb (b.exp-c.exp)) /\ a0_base<>0))
+    (ensures (let r=sub1sp_exact b c in
+              let cnt=64-(nbits a0_base) in
+        normal_fp_cond r /\
+        a0_base*pow2 64+sb_1=r.limb*pow2 (64-(b.exp-c.exp)) /\
+        b.exp-cnt =(high_mant r p).exp
+    ))
+
+#set-options "--z3rlimit 400"
+
+let lemma_sub1sp1_gt_branch_1_a0_bx b c p sb_1 a0_base=
+    lemma_gt_exp_sub1sp b c;
+    let r=sub1sp_exact b c in
+    let cnt=64-(nbits a0_base) in
+    let d=b.exp-c.exp in
+    shift_left_value_lemma #64 c.limb (64-d);
+    shift_right_value_lemma #64 c.limb d;
+    lemma_multiple_div c.limb (pow2 (64-d));
+    assert(shift_right #64 c.limb d=(c.limb*pow2 (64-d) / pow2 (64-d) / pow2 d));
+    lemma_div_div (c.limb*pow2 (64-d)) (pow2 (64-d)) (pow2 d);
+    lemma_pow2_mul (64-d) d;
+    lemma_euclidean (c.limb*pow2 (64-d)) (pow2 64);
+    assert(b.limb*pow2 64-c.limb*(pow2 (64-d))=a0_base*pow2 64+sb_1);
+    lemma_distr_sub_left (b.limb*pow2 d) c.limb (pow2 64-d);
+    assert((b.limb*pow2 d-c.limb)*(pow2 (64-d))=a0_base*pow2 64+sb_1);
+    lemma_fp_exp_ge b c;
+    assert(sub1sp_gt_limb b c=(b.limb*pow2 d-c.limb));
+
+    lemma_nbits_pow2_add a0_base 64 sb_1;
+    lemma_nbits_pow2_mul r.limb (64-d);
+
+    assert(nbits (r.limb*(pow2 (64-d)))=nbits a0_base+64);
+    assert(r.len=nbits (r.limb*(pow2 (64-d)))-(64-d));
+    assert(nbits r.limb=nbits a0_base+d)
+
+#set-options "--z3rlimit 100"
