code/experimental/mpfr/MPFR.Sub1sp1.fst
@@ -1,0 +1,422 @@
+module MPFR.Sub1sp1
+
+open FStar.HyperStack.All
+open FStar.HyperStack
+open FStar.HyperStack.ST
+open FStar.Buffer
+open FStar.UInt64
+open FStar.UInt
+open FStar.Int.Cast
+open FStar.Mul
+open MPFR.Dyadic
+open MPFR.Spec.Lib
+open MPFR.Spec.Sub1
+open MPFR.Spec.Round
+open MPFR.Maths
+
+open MPFR.Lib
+open MPFR.Exceptions
+
+open MPFR.Exceptions.Lemma
+open MPFR.Sub1sp1.Lemma
+open MPFR.Add1sp1
+open MPFR.Add1sp1.Lemma
+
+module ST = FStar.HyperStack.ST
+module I32 = FStar.Int32
+module I64 = FStar.Int64
+module U32 = FStar.UInt32
+
+#set-options "--z3refresh --z3rlimit 100 --max_fuel 1 --initial_fuel 0 --max_ifuel 1 --initial_ifuel 0"
+
+let mpfr_sub1sp1_post_cond h0 t h1 (a:mpfr_ptr) b c (p:mpfr_reg_prec_t) rnd_mode exact: GTot Type0=
+        (* Memory safety *)
+        mpfr_live h1 a /\ mpfr_live h1 b /\ mpfr_live h1 c /\
+        mpfr_disjoint_or_equal h1 a b /\ mpfr_disjoint_or_equal h1 a c /\
+        mpfr_disjoint_or_equal h1 b c /\ mpfr_modifies a h0 h1 /\
+        (* Functional correctness *)
+        mpfr_valid_cond h1 a /\
+        mpfr_round_cond exact (I64.v p) rnd_mode (as_fp h1 a) /\
+        mpfr_ternary_cond (I32.v t) exact (as_fp h1 a)
+
+inline_for_extraction 
+val count_leading_zeros: a:u64{not (a=^0uL)}->Tot (cnt:u32{U32.v cnt<32 /\ v (a<<^cnt)>=pow2 63 /\ v a*pow2 (U32.v cnt)<pow2 64 /\ U32.v cnt=64-(nbits (v a))})
+
+let count_leading_zeros a = MPFR.Lib.Clz.count_leading_zeros a
+
+inline_for_extraction val mpfr_sub1sp1_eq_branch_1:
+    a:mpfr_ptr -> b:mpfr_ptr -> c:mpfr_ptr ->
+    ap:buffer mp_limb_t -> bp:buffer mp_limb_t -> cp:buffer mp_limb_t ->
+    bx:mpfr_reg_exp_t ->cx:mpfr_reg_exp_t
+    ->rnd_mode:mpfr_rnd_t->
+    p:mpfr_reg_prec_t -> sh:mpfr_reg_prec_t -> Stack i32
+    (requires (fun h->mpfr_sub1sp1_pre_cond h a b c p /\
+    mpfr_sub1sp1_pre_cond_2 h a b c bx cx ap bp cp p sh /\
+    I64.(bx=^cx) /\ as_val h bp=as_val h cp 
+    ))
+ (ensures (fun h0 t h1 -> 
+   let exact=sub1sp_exact (as_fp h0 b) (as_fp h0 c) in 
+   mpfr_sub1sp1_post_cond h0 t h1 a b c p rnd_mode exact))
+
+let mpfr_sub1sp1_eq_branch_1 a b c ap bp cp bx cx rnd_mode p sh=
+    if rnd_mode=MPFR_RNDD then mpfr_SET_NEG a else mpfr_SET_POS a;
+    mpfr_SET_ZERO a;
+    mpfr_RET 0l
+
+let mpfr_sub1sp1_any_post_cond h0 s h1 (a:mpfr_ptr) b c (p:mpfr_reg_prec_t) exact: GTot Type0=
+        (* Memory safety *)
+        mpfr_live h1 a /\ mpfr_live h1 b /\ mpfr_live h1 c /\
+        length (as_struct h1 a).mpfr_d = 1 /\
+        length (as_struct h1 b).mpfr_d = 1 /\ length (as_struct h1 c).mpfr_d = 1 /\
+        normal_cond h1 a /\ 
+        (as_normal h1 a).prec=I64.v p /\  (as_struct h0 a).mpfr_d==(as_struct h1 a).mpfr_d /\
+        (*Functional correctness*)
+        I64.(v ((as_struct h0 a).mpfr_prec)=v p) /\
+        I64.(v ((as_struct h0 b).mpfr_prec)=v p) /\
+        I64.(v ((as_struct h0 c).mpfr_prec)=v p) /\
+        mpfr_reg_cond h0 b /\ mpfr_reg_cond h0 c /\
+        (let r = sub1sp_exact (as_reg_fp h0 b) (as_reg_fp h0 c) in
+        normal_fp_cond r /\
+        I64.(s.bx<=^mpfr_EMAX) /\
+        as_val h1 (as_struct h1 a).mpfr_d * pow2 (high_mant r (I64.v p)).len = (high_mant r (I64.v p)).limb * (pow2 64) /\
+        I64.v s.sh = I64.v gmp_NUMB_BITS - I64.v p /\
+        I64.v s.bx = (high_mant r (I64.v p)).exp /\
+        (rb_def r (I64.v p) = (v s.rb <> 0)) /\
+        (sb_def r (I64.v p) = (v s.sb <> 0)))
+
+inline_for_extraction val mpfr_sub1sp1_eq:
+    a:mpfr_ptr -> b:mpfr_ptr -> c:mpfr_ptr ->
+    ap:buffer mp_limb_t -> bp:buffer mp_limb_t -> cp:buffer mp_limb_t ->
+    bx:mpfr_reg_exp_t -> cx:mpfr_reg_exp_t ->
+    p:mpfr_reg_prec_t -> sh:mpfr_reg_prec_t -> Stack state
+    (requires (fun h-> mpfr_sub1sp1_pre_cond h a b c p /\
+    mpfr_sub1sp1_pre_cond_2 h a b c bx cx ap bp cp p sh /\
+    I64.(bx=^cx) /\
+    I64.(as_val h bp<>as_val h cp)
+    ))
+    (ensures (fun h0 s h1->
+    let exact=sub1sp_exact (as_fp h0 b) (as_fp h0 c) in
+    mpfr_sub1sp1_any_post_cond h0 s h1 a b c p exact /\
+    modifies_2 a (as_struct h1 a).mpfr_d h0 h1 /\
+    mpfr_modifies a h0 h1 /\
+    (as_normal h1 a).sign=exact.sign))
+
+let mpfr_sub1sp1_eq a b c ap bp cp bx cx p sh =
+    let h0=ST.get() in
+    let vb= v bp.(0ul) in
+    let vc= v cp.(0ul) in
+    let vsh= I64.(v sh) in 
+    if(cp.(0ul)>^bp.(0ul)) then begin 
+      let a0=cp.(0ul) -^ bp.(0ul) in
+      let cnt=count_leading_zeros a0 in
+      mpfr_SET_SIGN a (mpfr_NEG_SIGN (mpfr_SIGN b));(*mpfr_SET_OPPOSITE_SIGN does exactly this, but makes it harder to check*)
+      ap.(0ul) <- a0<<^cnt;
+      lemma_mod_distr_sub_zero vc vb (pow2 vsh);
+      lemma_shift_left_mod_pow2 a0 cnt vsh;
+      let bx=I64.(bx -^ (uint32_to_int64 cnt)) in
+      let h1=ST.get() in
+      shift_left_value_lemma (v a0) (U32.v cnt);
+      lemma_small_mod (v a0*pow2 (U32.v cnt)) (pow2 64);
+      mpfr_sub1sp1_eq_value_lemma ({(as_normal h1 a) with exp=I64.v bx}) (as_reg_fp h0 b) (as_reg_fp h0 c) (U32.v cnt) (I64.v p);
+      mpfr_sub1sp1_eq_rb_sb_lemma (as_reg_fp h0 b) (as_reg_fp h0 c) (I64.v p);
+      mk_state sh bx 0uL 0uL
+    end else begin
+      let a0=bp.(0ul) -^ cp.(0ul) in
+      let cnt=count_leading_zeros a0 in
+      mpfr_SET_SAME_SIGN a b;
+      ap.(0ul) <- a0<<^cnt;
+      lemma_mod_distr_sub_zero vb vc (pow2 vsh);
+      lemma_shift_left_mod_pow2 a0 cnt vsh;
+      let bx=I64.(bx -^ (uint32_to_int64 cnt)) in
+      let h1=ST.get() in
+      shift_left_value_lemma (v a0) (U32.v cnt);
+      lemma_small_mod (v a0*pow2 (U32.v cnt)) (pow2 64);
+      mpfr_sub1sp1_eq_value_lemma ({(as_normal h1 a) with exp=I64.v bx}) (as_reg_fp h0 b) (as_reg_fp h0 c) (U32.v cnt) (I64.v p);
+      mpfr_sub1sp1_eq_rb_sb_lemma (as_reg_fp h0 b) (as_reg_fp h0 c) (I64.v p);
+      mk_state sh bx 0uL 0uL
+    end
+
+val mpfr_sub1sp1_gt_branch_1:  a:mpfr_ptr -> b:mpfr_ptr -> c:mpfr_ptr ->
+    ap:buffer mp_limb_t -> bp:buffer mp_limb_t -> cp:buffer mp_limb_t ->
+    bx:mpfr_reg_exp_t ->cx:mpfr_reg_exp_t ->
+    p:mpfr_reg_prec_t -> sh:mpfr_reg_prec_t ->
+    mask:u64 -> sb_1:u64 -> a0_base:u64 -> Stack state
+    (requires (fun h->
+    v a0_base<>0 /\
+    v mask=pow2 (I64.v sh)-1 /\
+    I64.(v (bx -^ cx))<64 /\
+    mpfr_sub1sp1_pre_cond h a b c p /\
+    mpfr_sub1sp1_pre_cond_2 h a b c bx cx ap bp cp p sh /\
+    I64.(bx>^cx) /\
+    v sb_1=add_mod #64 (pow2 64-1-(shift_left #64 (as_val h cp) (64-I64.(v (bx -^ cx))))) 1 /\
+    v a0_base=((as_val h bp)-(if (v sb_1)=0 then 0 else 1))-(shift_right #64 (as_val h cp) I64.(v (bx -^ cx))) ))
+    (ensures (fun h0 s h1->
+    let exact=sub1sp_exact (as_fp h0 b) (as_fp h0 c) in
+    mpfr_sub1sp1_any_post_cond h0 s h1 a b c p exact /\
+    modifies_1 (as_struct h1 a).mpfr_d h0 h1))
+
+#set-options "--z3rlimit 400"
+
+let mpfr_sub1sp1_gt_branch_1 a b c ap bp cp bx cx p sh mask sb_1 a0_base=
+    let h0=ST.get() in
+    lemma_gt_exp_sub1sp (as_reg_fp h0 b) (as_reg_fp h0 c);
+    let cnt=count_leading_zeros a0_base in
+    let a0=if U32.(cnt =^ 0ul) then a0_base else
+    (a0_base <<^ cnt) |^ (sb_1 >>^ U32.(64ul -^ cnt)) in
+    let sb_2=sb_1 <<^ cnt in
+    let rb=a0 &^ (mpfr_LIMB_ONE <<^ (int64_to_uint32 I64.(sh-^1L))) in
+    let sb=sb_2 |^ ((a0 &^ mask) ^^ rb) in
+    ap.(0ul) <- a0 &^ (UInt64.lognot mask);
+
+    lemma_nth_top_bit (v (a0_base <<^ cnt));
+    lemma_lognot_value mask;
+    lemma_pow2_le (I64.v sh) 63;
+    lemma_nth_top_bit (v (UInt64.lognot mask));
+    lemma_nth_top_bit (v (a0 &^ (UInt64.lognot mask)));
+    lemma_lognot_mask_mod a0 mask (I64.v sh);
+
+    (let r=sub1sp_exact (as_reg_fp h0 b) (as_reg_fp h0 c) in
+    let d=I64.(v (bx-^cx)) in
+    let a0sb=(v a0)*pow2 64+(v sb_2) in
+    lemma_sub1sp1_gt_branch_1_a0_bx (as_reg_fp h0 b) (as_reg_fp h0 c) (I64.v p) (v sb_1) (v a0_base);
+    lemma_shift_left_dp (v a0_base) (v sb_1) U32.(v cnt);
+    assert((v a0)*pow2 64+(v sb_2)=((v a0_base)*pow2 64+(v sb_1))*pow2 U32.(v cnt));
+    assert((v a0_base)*pow2 64+(v sb_1)=r.limb*pow2(64-d));
+    lemma_paren_mul_right r.limb (pow2 (64-d)) (pow2 U32.(v cnt));
+    lemma_pow2_mul (64-d) U32.(v cnt);
+    assert(a0sb=r.limb*pow2 (128-r.len));
+    lemma_sub1sp1_gt_branch_1_rb_sb_value r (v a0) (v sb_2) (v mask) (I64.v p)
+    );
+    mk_state sh I64.(bx-^(uint32_to_int64 cnt)) rb sb
+
+inline_for_extraction val mpfr_sub1sp1_gt:
+    a:mpfr_ptr -> b:mpfr_ptr -> c:mpfr_ptr ->
+    ap:buffer mp_limb_t -> bp:buffer mp_limb_t -> cp:buffer mp_limb_t ->
+    bx:mpfr_reg_exp_t ->cx:mpfr_reg_exp_t ->
+    p:mpfr_reg_prec_t -> sh:mpfr_reg_prec_t -> Stack state
+    (requires (fun h->
+    mpfr_sub1sp1_pre_cond h a b c p /\
+    mpfr_sub1sp1_pre_cond_2 h a b c bx cx ap bp cp p sh /\
+    I64.(bx>^cx)))
+    (ensures (fun h0 s h1->
+    let exact=sub1sp_exact (as_fp h0 b) (as_fp h0 c) in
+    mpfr_sub1sp1_any_post_cond h0 s h1 a b c p exact /\
+    modifies_1 (as_struct h1 a).mpfr_d h0 h1))
+
+let mpfr_sub1sp1_gt a b c ap bp cp bx cx p sh =
+    let h0=ST.get() in
+    let d=I64.(bx-^cx) in
+    let bp0ul=bp.(0ul) in
+    let cp0ul=cp.(0ul) in
+    let mask=mpfr_LIMB_MASK (int64_to_uint32 sh) in
+    lemma_gt_exp_sub1sp (as_reg_fp h0 b) (as_reg_fp h0 c);
+    if(I64.(d<^64L)) then begin
+      let sb_1=UInt64.minus (cp0ul<<^(int64_to_uint32 I64.(gmp_NUMB_BITS -^ d))) in
+      lemma_lognot_value (cp0ul<<^(int64_to_uint32 I64.(gmp_NUMB_BITS -^ d)));
+      assert(v sb_1=add_mod #64 (pow2 64-1-(shift_left #64 (v cp0ul) (64-I64.v d))) 1);
+      assert(v cp0ul%(pow2 (I64.v sh))=0);
+      lemma_pow2_mod_mod_zero (v cp0ul) (I64.v sh) 1;
+      lemma_sub1sp1_gt_1_valid bp0ul cp0ul d;
+      mpfr_sub1sp1_gt_branch_1 a b c ap bp cp bx cx p sh mask sb_1 (bp0ul -^ (if sb_1=^0uL then 0uL else 1uL) -^ (cp0ul >>^ (int64_to_uint32 d)))
+    end else begin 
+      if(bp0ul>^mpfr_LIMB_HIGHBIT) then begin
+        assert((v bp0ul)%(pow2 (I64.v sh))=0);
+        lemma_mod_ge_zero (v bp0ul) (pow2 (I64.v sh));
+        lemma_pow2_mod 63 (I64.v sh);
+        lemma_mod_distr_sub_zero (v bp0ul) (v mpfr_LIMB_HIGHBIT) (pow2 (I64.v sh));
+        lemma_mod_ge_zero (v bp0ul-v mpfr_LIMB_HIGHBIT) (pow2 (I64.v sh));
+        assert(bp0ul -^ mpfr_LIMB_HIGHBIT >=^ (mpfr_LIMB_ONE <<^ (int64_to_uint32 sh)));
+        assert((bp0ul -^ (mpfr_LIMB_ONE <<^ (int64_to_uint32 sh)))>=^mpfr_LIMB_HIGHBIT);
+        ap.(0ul) <- bp0ul -^ (mpfr_LIMB_ONE <<^ (int64_to_uint32 sh));
+        let h1=ST.get() in
+        shift_left_value_lemma (v mpfr_LIMB_ONE) (I64.v sh);
+        lemma_pow2_mul_mod (v mpfr_LIMB_ONE) (I64.v sh) 64;
+        lemma_multiple_mod (v mpfr_LIMB_ONE%pow2 (64-(I64.v sh))) (pow2 (I64.v sh));
+        lemma_mod_distr_sub_zero (v bp0ul) (v (mpfr_LIMB_ONE <<^ (int64_to_uint32 sh))) (pow2 (I64.v sh));
+        lemma_sub1sp1_gt_rb_sb_exp_2 (as_reg_fp h0 b) (as_reg_fp h0 c) (I64.v p);
+        lemma_sub1sp1_gt_value_2 (as_reg_fp h0 b) (as_reg_fp h0 c) (I64.v p);
+        mk_state sh bx 1uL 1uL
+      end else begin
+        let rb=(I64.(sh>^1L||d>^gmp_NUMB_BITS)||cp0ul=mpfr_LIMB_HIGHBIT) in
+        let sb=(I64.(sh>^1L||d>^gmp_NUMB_BITS)||cp0ul<>mpfr_LIMB_HIGHBIT) in
+        ap.(0ul) <- (UInt64.lognot mask);
+        let h1=ST.get() in
+        lemma_lognot_value mask;
+        lemma_pow2_mod 64 (I64.v sh);
+        lemma_mod_distr_sub_zero (pow2 64) (pow2 (I64.v sh)) (pow2 (I64.v sh));
+        lemma_sub1sp1_gt_rb_sb_exp_3 (as_reg_fp h0 b) (as_reg_fp h0 c) (I64.v p);
+        lemma_sub1sp1_gt_value_3 (as_reg_fp h0 b) (as_reg_fp h0 c) (I64.v p);
+        assert(I64.(v (bx-^1L))=(sub1sp_exact (as_reg_fp h0 b) (as_reg_fp h0 c)).exp);
+        mk_state sh I64.(bx-^1L) (if rb then 1uL else 0uL) (if sb then 1uL else 0uL)
+      end
+    end
+
+#set-options "--z3rlimit 100"
+
+(* specifications for mpfr_sub1sp1 *)
+val mpfr_sub1sp1: a:mpfr_ptr -> b:mpfr_ptr -> c:mpfr_ptr ->
+                  rnd_mode:mpfr_rnd_t -> p:mpfr_prec_t -> Stack i32
+    (requires (fun h -> mpfr_sub1sp1_pre_cond h a b c p))
+    (ensures  (fun h0 t h1 ->
+    let exact=sub1sp_exact (as_fp h0 b) (as_fp h0 c) in
+    mpfr_sub1sp1_post_cond h0 t h1 a b c p rnd_mode exact))
+
+inline_for_extraction val mpfr_sub1sp1_any:
+    a:mpfr_ptr -> b:mpfr_ptr -> c:mpfr_ptr ->
+    ap:buffer mp_limb_t -> bp:buffer mp_limb_t -> cp:buffer mp_limb_t ->
+    bx:mpfr_reg_exp_t -> cx:mpfr_reg_exp_t ->
+    p:mpfr_reg_prec_t -> sh:mpfr_reg_prec_t -> Stack state
+    (requires (fun h-> mpfr_sub1sp1_pre_cond h a b c p /\
+    mpfr_sub1sp1_pre_cond_2 h a b c bx cx ap bp cp p sh /\
+    (I64.(~(bx=^cx)) \/ I64.(as_val h bp<>as_val h cp))
+    ))
+    (ensures (fun h0 s h1->
+    let exact=sub1sp_exact (as_fp h0 b) (as_fp h0 c) in
+    mpfr_sub1sp1_any_post_cond h0 s h1 a b c p exact /\
+    modifies_2 a (as_struct h1 a).mpfr_d h0 h1 /\
+    mpfr_modifies a h0 h1 /\
+    (as_normal h1 a).sign=exact.sign))
+
+let mpfr_sub1sp1_any a b c ap bp cp bx cx p sh =
+    let h0=ST.get() in
+    if I64.(bx =^ cx) then begin
+      mpfr_sub1sp1_eq a b c ap bp cp bx cx p sh
+    end else begin 
+    let b,c,bx,cx,bp,cp=(if I64.(bx >=^ cx)
+    then (mpfr_SET_SAME_SIGN a b;lemma_gt_exp_sub1sp (as_fp h0 b) (as_fp h0 c);b,c,bx,cx,bp,cp)
+    else (mpfr_SET_SIGN a (mpfr_NEG_SIGN (mpfr_SIGN b));lemma_gt_exp_sub1sp (as_fp h0 c) (as_fp h0 b);c,b,cx,bx,cp,bp)) in       
+    mpfr_sub1sp1_gt a b c ap bp cp bx cx p sh
+    end
+
+val lemma_eval_small_exp: r:normal_fp -> emax:int -> Lemma
+    (requires r.exp<emax)
+    (ensures eval_abs r<.(mk_dyadic 1 (emax-1)))
+    
+let lemma_eval_small_exp r emax=
+assert((mk_dyadic 1 r.exp) <=. (mk_dyadic 1 (emax-1)));
+assert(eval_abs r<. (mk_dyadic 1 r.exp))
+
+val lemma_dyadic_pow2: k:nat -> e:int -> Lemma
+    ((mk_dyadic (pow2 k) e) =. mk_dyadic 1 (k+e))
+
+let lemma_dyadic_pow2 k e=()
+
+val lemma_underflow_low_prec: b:mpfr_reg_fp -> c:mpfr_reg_fp{b.prec=c.prec} -> r:normal_fp -> Lemma
+    (requires (r==sub1sp_exact b c /\ r.exp<mpfr_EMIN_spec))
+    (ensures (r.prec<b.prec))
+
+let lemma_underflow_low_prec b c r=()
+
+val lemma_eval_abs_zero: a:valid_fp{a.limb=0} -> r:valid_fp{r.limb<>0} -> Lemma
+    (ensures (eval_abs a <. eval_abs r))
+
+let lemma_eval_abs_zero a r=()
+
+val lemma_sub1sp1_rndn_eval: r:normal_fp{mpfr_PREC_COND r.prec /\ r.prec<=128} -> Lemma
+    (requires (r.exp<mpfr_EMIN_spec-1 \/ (r.exp=mpfr_EMIN_spec-1 /\ r.limb=pow2 (r.len-1)) ))
+    (ensures  (eval_abs r <=. fdiv_pow2 (mpfr_underflow_bound r.prec) 1 /\
+               eval_abs r <. mpfr_overflow_bound r.prec))
+
+let lemma_sub1sp1_rndn_eval r=
+    if r.exp=mpfr_EMIN_spec-1 then begin
+        lemma_dyadic_pow2 (r.len-1) (r.exp-r.len);
+        assert(eval_abs r <=. mk_dyadic 1 (mpfr_EMIN_spec-2))
+    end
+    else begin
+        lemma_dyadic_pow2 r.len (r.exp-r.len);
+        dyadic_le_exp_lemma r.exp (mpfr_EMIN_spec-2);
+        assert(eval_abs r <=. mk_dyadic 1 (mpfr_EMIN_spec-2))
+    end;
+    let l = prec_to_len r.prec in
+    lemma_dyadic_pow2 (l-1) (mpfr_EMIN_spec-l-1);
+    lemma_pow2_lt (l-r.prec) l;
+    dyadic_le_limb_lemma 1 (pow2 l-pow2 (l-r.prec)) (mpfr_EMAX_spec-l);
+    assert(mk_dyadic 1 (mpfr_EMAX_spec-l) <=. mpfr_overflow_bound r.prec);
+    assert(mpfr_EMIN_spec-2<mpfr_EMAX_spec-l);
+    assert(fdiv_pow2 (mpfr_underflow_bound r.prec) 1 <=. mk_dyadic 1 (mpfr_EMIN_spec-2));
+    dyadic_lt_exp_lemma (mpfr_EMIN_spec-2) (mpfr_EMAX_spec-l);
+    assert(fdiv_pow2 (mpfr_underflow_bound r.prec) 1 <. mpfr_overflow_bound r.prec)
+
+#set-options "--z3rlimit 400"
+
+let mpfr_sub1sp1 a b c rnd_mode p =
+    let bx=mpfr_GET_EXP b in
+    let cx=mpfr_GET_EXP c in
+    let ap=mpfr_MANT a in
+    let bp=mpfr_MANT b in
+    let cp=mpfr_MANT c in
+    let sh=I64.(gmp_NUMB_BITS -^ p) in
+    let bp0ul=bp.(0ul) in
+    let cp0ul=cp.(0ul) in
+    let h0=ST.get() in
+    if I64.(bx =^ cx) && (bp0ul=cp0ul) then
+       mpfr_sub1sp1_eq_branch_1 a b c ap bp cp bx cx rnd_mode p sh
+    else begin
+    let st=mpfr_sub1sp1_any a b c ap bp cp bx cx p sh in
+    let h1 = ST.get() in
+    if I64.(st.bx <^ mpfr_EMIN) then begin 
+        let s = mpfr_SIGN a in
+        let ap0ul=ap.(0ul) in
+        if(rnd_mode=MPFR_RNDN&&(I64.(st.bx<^(mpfr_EMIN-^1L))||ap0ul=mpfr_LIMB_HIGHBIT)) then begin
+            mpfr_SET_ZERO a;
+            let h2=ST.get() in
+            (let r=(sub1sp_exact (as_reg_fp h0 b) (as_reg_fp h0 c)) in
+            let p=I64.v p in
+            lemma_underflow_low_prec (as_reg_fp h0 b) (as_reg_fp h0 c) r;
+            let hm=high_mant r p in
+            assert(eval_abs r =. eval_abs hm);
+            if hm.exp=mpfr_EMIN_spec-1 then begin
+                lemma_pow2_mul 63 hm.len;
+                lemma_pow2_mul (hm.len-1) 64;
+                assert(hm.limb=pow2 (hm.len-1))
+            end;
+            assert(hm.prec<=128);
+            lemma_sub1sp1_rndn_eval hm;
+            assert(eval_abs r =. eval_abs (round_def r p MPFR_RNDN));
+            let a=(as_fp h2 a) in
+            lemma_eval_abs_zero a r;
+            if r.sign>0 then
+                eval_lt_intro_lemma a r
+            else
+                eval_lt_intro_lemma r a
+            );
+            mpfr_NEG_SIGN s
+        end else begin 
+            let h1b=ST.get() in
+            let t=mpfr_underflow a rnd_mode s in
+            let h2=ST.get() in
+            (let r=(sub1sp_exact (as_reg_fp h0 b) (as_reg_fp h0 c)) in
+            let p=(I64.v p) in
+            lemma_underflow_low_prec (as_reg_fp h0 b) (as_reg_fp h0 c) r;
+            if rnd_mode=MPFR_RNDN then begin
+                let hm=high_mant r p in
+                assert(eval_abs r =. eval_abs hm);
+                lemma_mul_lt_right (pow2 hm.len) (pow2 63) (v ap0ul);
+                lemma_pow2_mul 63 hm.len;
+                lemma_pow2_mul (hm.len-1) 64;
+                lemma_dyadic_pow2 (hm.len-1) (hm.exp-hm.len);
+                assert (eval_abs hm >. mk_dyadic 1 (mpfr_EMIN_spec-2));
+                lemma_dyadic_pow2 ((prec_to_len p)-1) (mpfr_EMIN_spec-(prec_to_len p)-1);
+                assert(eval_abs hm >. fdiv_pow2 (mpfr_underflow_bound p) 1);
+                assert(eval_abs r >. fdiv_pow2 (mpfr_underflow_bound p) 1)
+            end;
+            assert(eval_abs r =. eval_abs (round_def r p MPFR_RNDN));
+            assert( (MPFR_RNDN? rnd_mode ==> eval_abs r >. fdiv_pow2 (mpfr_underflow_bound p) 1));
+            lemma_eval_small_exp r mpfr_EMIN_spec;
+            lemma_dyadic_pow2 ((prec_to_len p)-1) (mpfr_EMIN_spec-(prec_to_len p));
+            assert(eval_abs r =. eval_abs (round_def r p rnd_mode));
+            assert(eval_abs (round_def r p rnd_mode) <. mpfr_underflow_bound p);
+            mpfr_underflow_post_cond_lemma r p rnd_mode (I32.v t) (as_fp h2 a)
+            );
+            assert (modifies_0 h1 h1b);
+            mpfr_modifies_trans_lemma a h0 h1 h2;
+            t
+        end
+    end else begin
+        let t = mpfr_add1sp1_round a ap rnd_mode st in
+	let h2 = ST.get() in
+	mpfr_add1sp1_round_post_cond_lemma (sub1sp_exact (as_reg_fp h0 b) (as_reg_fp h0 c)) (I64.v (as_struct h0 a).mpfr_prec) (as_normal_ h1 ({as_struct h1 a with mpfr_exp = st.bx})) (st.rb <> 0uL) (st.sb <> 0uL) rnd_mode (I32.v t) (as_fp h2 a); 
+	mpfr_modifies_trans_lemma a h0 h1 h2;
+	t
+    end
+    end
