code/experimental/mpfr/Test.MPFR.fst
@@ -1,0 +1,143 @@
+module Test.MPFR
+
+open FStar.HyperStack.All
+//open FStar.HyperStack.IO
+open FStar.Buffer
+
+module U64 = FStar.UInt64
+module U32 = FStar.UInt32
+module I64 = FStar.Int64
+module I32 = FStar.Int32
+
+open MPFR.Lib
+open MPFR.RoundingMode
+open MPFR
+
+#set-options "--z3refresh --lax --max_fuel 1 --initial_fuel 0 --max_ifuel 1 --initial_ifuel 0"
+
+//inline_for_extraction noextract
+//let cprint x = C.String.print (C.String.of_literal x)
+//let cprint x = (*C.String.print (C.String.of_literal x)*) print_string x //Printf.printf "%s" x
+
+// inline_for_extraction noextract
+// let print_i32 x = cprint (string_of_int (I32.v x)); cprint " "
+// inline_for_extraction noextract
+// let print_i64 x = cprint (string_of_int (I64.v x)); cprint " "
+// inline_for_extraction noextract
+// let print_u64 x = cprint (string_of_int (U64.v x)); cprint " "
+
+// inline_for_extraction noextract
+// let print_rnd rnd = match rnd with
+//     | MPFR_RNDN -> cprint "MPFR_RNDN "
+//     | MPFR_RNDZ -> cprint "MPFR_RNDZ "
+//     | MPFR_RNDA -> cprint "MPFR_RNDA "
+//     | MPFR_RNDU -> cprint "MPFR_RNDU "
+//     | MPFR_RNDD -> cprint "MPFR_RNDD "
+ 
+
+
+val test_add1sp1: mpfr_sign_t -> mp_limb_t -> mpfr_exp_t -> mp_limb_t -> mpfr_exp_t -> mpfr_rnd_t ->
+    mpfr_prec_t -> mp_limb_t -> mpfr_exp_t -> I32.t -> ST bool
+    (requires (fun h -> True))
+    (ensures  (fun h0 r h1 -> True))
+
+let test_add1sp1 s bp bx cp cx rnd_mode p rp rx rt =
+    C.String.print (C.String.of_literal "Testing add1sp1: \n");
+    //print_i32 s; print_u64 bp; print_i64 bx; print_u64 cp; print_i64 cx; print_rnd rnd_mode;
+    //print_i64 p; print_u64 rp; print_i64 rx; print_i32 rt;
+    //cprint "\n";
+    push_frame();
+    let bm = createL [bp] in
+    let bs = mk_mpfr_struct p s bx bm in
+    let b = createL [bs] in
+    let cm = createL [cp] in
+    let cs = mk_mpfr_struct p s cx cm in
+    let c = createL [cs] in
+    let at = mpfr_add1sp1 c b c rnd_mode p in
+    let asign = mpfr_SIGN c in
+    let am = mpfr_MANT c in
+    let ap = am.(0ul) in
+    let ax = mpfr_EXP c in
+    pop_frame ();
+    C.String.print (C.String.of_literal "Result: \n");
+    // print_i32 asign;
+    // print_u64 ap;
+    // print_i64 ax;
+    // print_i32 at;
+    if ((U64.(ap =^ rp) && I64.(ax =^ rx)) || (I64.(ax =^ mpfr_EXP_INF) && I64.(ax =^ rx))) &&
+         I32.(asign =^ s) && I32.(at =^ rt) then begin
+        C.String.print (C.String.of_literal "YES!!!\n");
+	true
+    end else begin
+        C.String.print (C.String.of_literal "no...\n");
+	false
+    end
+
+
+let test_sub1sp1 s bp bx cp cx rnd_mode p rp rx rt =
+    C.String.print (C.String.of_literal "Testing sub1sp1: \n");
+    //print_i32 s; print_u64 bp; print_i64 bx; print_u64 cp; print_i64 cx; print_rnd rnd_mode;
+    //print_i64 p; print_u64 rp; print_i64 rx; print_i32 rt;
+    //cprint "\n";
+    push_frame();
+    let bm = createL [bp] in
+    let bs = mk_mpfr_struct p s bx bm in
+    let b = createL [bs] in
+    let cm = createL [cp] in
+    let cs = mk_mpfr_struct p s cx cm in
+    let c = createL [cs] in
+    let at = mpfr_sub1sp1 c b c rnd_mode p in
+    let asign = mpfr_SIGN c in
+    let am = mpfr_MANT c in
+    let ap = am.(0ul) in
+    let ax = mpfr_EXP c in
+    pop_frame ();
+    C.String.print (C.String.of_literal "Result: \n");
+    // print_i32 asign;
+    // print_u64 ap;
+    // print_i64 ax;
+    // print_i32 at;
+    if ((U64.(ap =^ rp) && I64.(ax =^ rx)) || (I64.(ax =^ mpfr_EXP_INF) && I64.(ax =^ rx))) &&
+         I32.(asign =^ s) && I32.(at =^ rt) then begin
+        C.String.print (C.String.of_literal "YES!!!\n");
+	true
+    end else begin
+        C.String.print (C.String.of_literal "no...\n");
+	false
+    end
+
+let test1 () =
+    test_add1sp1 1l 9223372036854775808uL 53L 9223372036854775808uL 0L MPFR_RNDN 53L 9223372036854775808uL 53L (-1l)
+
+let test2 () =
+    test_add1sp1 (-1l) 9223372036854775808uL 0L 9223372036854775808uL 5L MPFR_RNDU 1L 9223372036854775808uL 5L 1l
+
+let test3 () =
+    test_add1sp1 1l 13835058055282163712uL 1073741823L 13835058055282163712uL 1073741822L MPFR_RNDN 2L 9223372036854779904uL mpfr_EXP_INF 1l
+
+let test4 () =
+    test_add1sp1 1l 11284843200441646272uL 12L 14910977271964212488uL (-1L) MPFR_RNDD 62L 11286663388096915340uL 12L (-1l)
+
+let tests1 () =
+    test_sub1sp1 1l 12105675798371893248uL 6L 9799832789158199296uL 5L MPFR_RNDN 63L 14411518807585587200uL 5L 0l
+
+val main: unit -> ST int
+    (requires (fun h -> True))
+    (ensures  (fun h0 r h1 -> True))
+
+let main () =
+    push_frame();
+    let t1 = test1 () in
+    let t2 = test2 () in
+    let t3 = test3 () in
+    let t4 = test4 () in
+  (*  let t1 = tests1 () in
+    let t2 = tests1 () in
+    let t3 = tests1 () in 
+    let t4 = tests1 () in *)
+    if t1 && t2 && t3 && t4 then
+        C.String.print (C.String.of_literal "\n === Congratulations!!! WE MADE IT!!! ===\n")
+    else
+        C.String.print (C.String.of_literal "\n I'm so sorry, but the tests failed...\n");
+    pop_frame();
+    0
